qed `auditor.CheckStart`

new/proof/github_com/sanjit_bhat/pav/auditor_proof/auditor.v
@@ -1,2 +1,134 @@
+From New.generatedproof.github_com.sanjit_bhat.pav Require Import auditor.
+
+From New.proof Require Import bytes sync.
+From New.proof.github_com.goose_lang Require Import std.
+From New.proof.github_com.sanjit_bhat.pav Require Import
+  advrpc cryptoffi hashchain ktcore merkle server.
+
+From New.proof.github_com.sanjit_bhat.pav.auditor_proof Require Import
+  base.
+
+(* TODO: bad New.proof.sync exports.
+https://github.com/mit-pdos/perennial/issues/470 *)
+From New.proof.github_com.sanjit_bhat.pav Require Import prelude.
+
 Module auditor.
+Import base.auditor.
+Section proof.
+Context `{hG: heapGS Σ, !ffi_semantics _ _, !globalsGS Σ} {go_ctx : GoContext}.
+
+Definition wish_CheckStart servPk reply (ep : w64) dig link : iProp Σ :=
+  ∃ digs0 digs1 cut,
+  (* hashchain. *)
+  "%Hlen_link_prev" ∷ ⌜Z.of_nat $ length reply.(server.StartReply.PrevLink) = cryptoffi.hash_len⌝ ∗
+  "#His_chain_prev" ∷ hashchain.is_chain digs0 cut reply.(server.StartReply.PrevLink)
+    (uint.nat reply.(server.StartReply.PrevEpochLen)) ∗
+  "%Hwish_chain" ∷ ⌜hashchain.wish_Verify reply.(server.StartReply.ChainProof) digs1⌝ ∗
+  "#His_chain_start" ∷ hashchain.is_chain (digs0 ++ digs1) cut link
+    (uint.nat reply.(server.StartReply.PrevEpochLen) + length digs1) ∗
+  "%Heq_ep" ∷ ⌜uint.Z reply.(server.StartReply.PrevEpochLen) + length digs1 - 1 = uint.Z ep⌝ ∗
+  "%Heq_dig" ∷ ⌜last digs1 = Some dig⌝ ∗
+  "#His_link_sig" ∷ ktcore.wish_VerifyLinkSig servPk ep link reply.(server.StartReply.LinkSig) ∗
+
+  (* vrf. *)
+  "#His_vrf_pk" ∷ cryptoffi.is_vrf_pk reply.(server.StartReply.VrfPk) ∗
+  "#His_vrf_sig" ∷ ktcore.wish_VerifyVrfSig servPk reply.(server.StartReply.VrfPk)
+    reply.(server.StartReply.VrfSig).
+
+Lemma wish_CheckStart_det pk r e0 e1 d0 d1 l0 l1 :
+  wish_CheckStart pk r e0 d0 l0 -∗
+  wish_CheckStart pk r e1 d1 l1 -∗
+  ⌜e0 = e1 ∧ d0 = d1 ∧ l0 = l1⌝.
+Proof.
+  iNamedSuffix 1 "0".
+  iNamedSuffix 1 "1".
+  iDestruct (hashchain.is_chain_inj with "His_chain_prev0 His_chain_prev1") as %[-> ->].
+  opose proof (hashchain.wish_Verify_det _ _ _ Hwish_chain0 Hwish_chain1) as ->.
+  iDestruct (hashchain.is_chain_det with "His_chain_start0 His_chain_start1") as %->.
+  iPureIntro.
+  rewrite Heq_dig0 in Heq_dig1.
+  rewrite Heq_ep0 in Heq_ep1.
+  by simplify_eq/=.
+Qed.
+
+Lemma wp_CheckStart sl_servPk servPk ptr_reply reply :
+  {{{
+    is_pkg_init auditor ∗
+    "#Hsl_servPk" ∷ sl_servPk ↦*□ servPk ∗
+    "#Hown_reply" ∷ server.StartReply.own ptr_reply reply (□)
+  }}}
+  @! auditor.CheckStart #sl_servPk #ptr_reply
+  {{{
+    (ep : w64) sl_dig sl_link ptr_vrfPk (err : bool),
+    RET (#ep, #sl_dig, #sl_link, #ptr_vrfPk, #err);
+    "Hgenie" ∷
+      match err with
+      | true => ¬ ∃ ep dig link, wish_CheckStart servPk reply ep dig link
+      | false =>
+        ∃ dig link,
+        "#Hsl_dig" ∷ sl_dig ↦*□ dig ∗
+        "#Hsl_link" ∷ sl_link ↦*□ link ∗
+        "#Hwish_CheckStart" ∷ wish_CheckStart servPk reply ep dig link ∗
+        "#Hown_vrf_pk" ∷ cryptoffi.own_vrf_pk ptr_vrfPk reply.(server.StartReply.VrfPk)
+      end
+  }}}.
+Proof.
+  wp_start as "@".
+  iNamed "Hown_reply". destruct reply. simpl.
+  wp_auto.
+  iDestruct (own_slice_len with "Hsl_PrevLink") as %[? _].
+  wp_if_destruct.
+  2: { iApply "HΦ". iIntros "@". simpl in *. word. }
+  iDestruct (hashchain.is_chain_invert PrevLink (uint.nat PrevEpochLen))
+    as "(%&%&#His_chain_prev)"; [word|].
+  wp_apply (hashchain.wp_Verify with "[$His_chain_prev]") as "* @".
+  { iFrame "#". }
+  wp_if_destruct.
+  { iApply "HΦ". iNamedSuffix 1 "'". simpl in *. iApply "Hgenie". naive_solver. }
+  iNamed "Hgenie".
+  iPersist "Hsl_newVal Hsl_newLink".
+  wp_if_destruct.
+  { iApply "HΦ". iNamedSuffix 1 "'". simpl in *.
+    opose proof (hashchain.wish_Verify_det _ _ _ Hwish_chain Hwish_chain') as ->.
+    apply last_Some in Heq_dig' as [? Heq].
+    apply (f_equal length) in Heq.
+    autorewrite with len in *.
+    word. }
+  wp_apply std.wp_SumNoOverflow.
+  wp_if_destruct.
+  2: { iApply "HΦ". iNamedSuffix 1 "'". simpl in *.
+    opose proof (hashchain.wish_Verify_det _ _ _ Hwish_chain Hwish_chain') as ->.
+    word. }
+  wp_apply ktcore.wp_VerifyLinkSig as "* @".
+  { iFrame "#". }
+  wp_if_destruct.
+  { iApply "HΦ". iNamedSuffix 1 "'". simpl in *. iApply "Hgenie".
+    opose proof (hashchain.wish_Verify_det _ _ _ Hwish_chain Hwish_chain') as ->.
+    iDestruct (hashchain.is_chain_inj with "His_chain_prev His_chain_prev'") as %[-> ->].
+    iDestruct (hashchain.is_chain_det with "His_chain His_chain_start'") as %->.
+    iExactEq "His_link_sig'". repeat f_equal. word. }
+  iNamed "Hgenie".
+  wp_apply cryptoffi.wp_VrfPublicKeyDecode as "* @ {Hsl_enc}".
+  { iFrame "#". }
+  wp_if_destruct.
+  { iApply "HΦ". iNamedSuffix 1 "'". simpl in *. by iApply "Hgenie". }
+  iNamed "Hgenie".
+  wp_apply ktcore.wp_VerifyVrfSig as "* @".
+  { iFrame "#". }
+  wp_if_destruct.
+  { iApply "HΦ". iNamedSuffix 1 "'". simpl in *. by iApply "Hgenie". }
+  iNamed "Hgenie".
+
+  iDestruct (cryptoffi.own_vrf_pk_valid with "Hown_vrf_pk") as "#His_vrf_pk".
+  iDestruct (hashchain.is_chain_hash_len with "His_chain_prev") as %?.
+  iApply "HΦ".
+  iFrame "#%". simpl in *.
+  iPureIntro. split; [word|].
+  destruct (last _) eqn:Heq; [done|].
+  apply last_None in Heq.
+  apply (f_equal length) in Heq.
+  simpl in *. word.
+Qed.
+
+End proof.
 End auditor.
